coq/Translation/cNNRCtoNNRC.v
@@ -1,0 +1,56 @@
+(*
+ * Copyright 2015-2016 IBM Corporation
+ *
+ * Licensed under the Apache License, Version 2.0 (the "License");
+ * you may not use this file except in compliance with the License.
+ * You may obtain a copy of the License at
+ *
+ * http://www.apache.org/licenses/LICENSE-2.0
+ *
+ * Unless required by applicable law or agreed to in writing, software
+ * distributed under the License is distributed on an "AS IS" BASIS,
+ * WITHOUT WARRANTIES OR CONDITIONS OF ANY KIND, either express or implied.
+ * See the License for the specific language governing permissions and
+ * limitations under the License.
+ *)
+
+Section cNNRCtoNNRC.
+  Require Import String.
+  Require Import List.
+  Require Import BasicRuntime.
+  Require Import cNNRC.
+  Require Import NNRC.
+
+  Context {fr:foreign_runtime}.
+
+  Section Top.
+    Context (h:brand_relation_t).
+
+    Definition nnrc_core_to_nnrc_top (q:nnrc_core) : nnrc :=
+      nnrc_core_to_nnrc q.
+
+    Theorem nnrc_core_to_nnrc_top_correct :
+      forall q:nnrc_core, forall global_env:bindings,
+          nnrc_core_eval_top h q global_env =
+          nnrc_eval_top h (nnrc_core_to_nnrc_top q) global_env.
+    Proof.
+      intros.
+      unfold nnrc_eval_top.
+      unfold nnrc_core_eval_top.
+      unfold nnrc_core_to_nnrc_top.
+      unfold lift_nnrc_core.
+      unfold nnrc_ext_eval.
+      destruct q; simpl.
+      rewrite core_nnrc_to_nnrc_ext_id.
+      reflexivity.
+      assumption.
+    Qed.
+  End Top.
+    
+End cNNRCtoNNRC.
+
+(* 
+*** Local Variables: ***
+*** coq-load-path: (("../../coq" "Qcert")) ***
+*** End: ***
+*)
